src/BinEncoders/take4/specs.v
@@ -1,0 +1,174 @@
+Require Import Coq.Strings.Ascii.
+Require Import Coq.Lists.List.
+
+Set Implicit Arguments.
+
+Definition bin := list bool.
+
+(* Notation "encode ⇹ decode" := *)
+Notation "encode <+> decode" :=
+  (forall data, decode (encode data) = data)
+    (at level 20, no associativity).
+
+(* Notation "encode ⇼ decode" := *)
+Notation "encode <++> decode" :=
+  (forall data ext, decode (encode data ++ ext) = (data, ext))
+    (at level 20, no associativity).
+
+Notation "<$ decode" :=
+  (forall bin, length (snd (decode bin)) <= pred (length bin))
+    (at level 20, no associativity).
+
+Class decoder
+      (A : Type)
+      (encode : A -> bin) :=
+  { decode : bin -> A;
+    decode_correct : encode <+> decode }.
+
+Class decoder_block
+      (A : Type)
+      (encode : A -> bin) :=
+  { decode_block : bin -> A * bin;
+    decode_block_app : encode <++> decode_block;
+    decode_block_wellfounded  : <$ decode_block }.
+
+Fixpoint exp2 (n : nat) :=
+  match n with
+  | O => S O
+  | S n' => exp2 n' + exp2 n'
+  end.
+
+Variable FixNat_encode : forall size, {n | n < exp2 size} -> bin.
+
+Global Instance FixNat_decoder
+       (size : nat)
+  : decoder_block (FixNat_encode size). Admitted.
+
+Variable List1_encode :
+  forall (A : Type) (encode_A : A -> bin) (size : nat),
+    {ls : list A | length ls < exp2 size} -> bin.
+
+Global Instance List1_decoder
+       (size : nat)
+       (A : Type)
+       (encode_A : A -> bin)
+       (A_Decoder : decoder_block encode_A)
+  : decoder_block (List1_encode encode_A size). Admitted.
+
+Record SSRecord :=
+  { field1 : { n | n < exp2 4 };
+    field2 : { ls : list { n | n < exp2 16 } | length ls < exp2 8 };
+    field3 : { n | n < exp2 2 } }.
+
+Definition SS_encode (s : SSRecord) :=
+  FixNat_encode _ (field1 s) ++
+  List1_encode (FixNat_encode _) _ (field2 s) ++
+  FixNat_encode _ (field3 s).
+
+Lemma decode_app_l (data_t proj_t prev_t : Type) :
+  forall (prev : data_t -> prev_t)
+         (proj : data_t -> proj_t)
+         (encode1 : proj_t -> bin)
+         (encode2 : data_t -> bin),
+  { decode : prev_t -> bin -> proj_t * bin |
+    forall data ext,
+      decode (prev data) (encode1 (proj data) ++ ext) = (proj data, ext) } ->
+  { decode : prev_t * proj_t -> bin -> data_t * bin |
+    forall data ext,
+      decode (prev data, proj data) (encode2 data ++ ext) = (data, ext) } ->
+  { decode : prev_t -> bin -> data_t * bin |
+    forall data ext,
+      decode (prev data) (encode1 (proj data) ++ encode2 data ++ ext) = (data, ext) }.
+Proof.
+  intros prev proj encode1 encode2.
+  destruct 1 as [ decode1 decode1_pf ]; destruct 1 as [ decode2 decode2_pf ].
+  eexists. intros data ext.
+  instantiate (1:=fun _prev _bin => let (_proj, _ext) := decode1 _prev _bin in
+                                    decode2 (_prev, _proj) _ext).
+  simpl. rewrite decode1_pf. rewrite decode2_pf. reflexivity.
+Qed.
+
+Lemma decode_inject_unit (T : Type) (P : T -> Prop) :
+  { decode : unit -> T | P (decode tt) } -> { decode : T | P decode }.
+Proof.
+  destruct 1; eauto.
+Qed.
+
+Lemma decode_resolve_hyp (data_t proj_t prev_t goal_t : Type) :
+  forall (prev : data_t -> prev_t)
+         (proj : data_t -> proj_t)
+         (goal : data_t -> goal_t)
+         (encode : proj_t -> bin),
+  { constr : prev_t -> proj_t -> goal_t |
+    forall data, constr (prev data) (proj data) = goal data } ->
+  { decode : bin -> proj_t * bin |
+    forall data ext, decode (encode data ++ ext) = (data, ext) } ->
+  { decode : prev_t -> bin -> goal_t * bin |
+    forall data ext,
+      decode (prev data) (encode (proj data) ++ ext) = (goal data, ext) }.
+Proof.
+  intros prev proj goal encode.
+  destruct 1 as [ constr constr_pf ]; destruct 1 as [ decode decode_pf ].
+  eexists. intros data ext.
+  instantiate (1:=fun _prev _bin => let (_proj, _ext) := decode _bin in
+                                    (constr _prev _proj, _ext)).
+  simpl. rewrite decode_pf. rewrite constr_pf. reflexivity.
+Qed.
+
+Lemma decode_generalize (data_t : Type) :
+  forall (encode : data_t -> bin),
+    { decode | encode <++> decode } -> { decode | encode <+> decode }.
+Proof.
+  intro encode. destruct 1 as [ decode decode_pf ].
+  eexists. instantiate (1:=fun _bin => fst (decode _bin)).
+  simpl. intro data.
+  rewrite <- app_nil_r with (l:=encode data). rewrite decode_pf. reflexivity.
+Qed.
+
+Lemma decode_app_assoc (data_t prev_t : Type) :
+  forall (prev : data_t -> prev_t)
+         (encode1 : data_t -> bin)
+         (encode2 : data_t -> bin),
+    { decode : prev_t -> bin -> data_t * bin |
+      forall data ext,
+        decode (prev data) (encode1 data ++ encode2 data ++ ext) = (data, ext) } ->
+    { decode : prev_t -> bin -> data_t * bin |
+      forall data ext,
+        decode (prev data) ((encode1 data ++ encode2 data) ++ ext) = (data, ext) }.
+Proof.
+  intros prev encode1 encode2.
+  destruct 1 as [ decode decode_pf ].
+  eexists. intros data ext.
+  instantiate (1:=decode). rewrite <- app_assoc. apply decode_pf.
+Qed.
+
+Definition SS_decode :
+  { decode : bin -> SSRecord | forall data, decode (SS_encode data) = data }.
+Proof.
+  unfold SS_encode.
+
+  eapply decode_generalize.
+  eapply decode_inject_unit.
+
+  eapply decode_app_assoc.
+  eapply decode_app_l.
+
+  eapply decode_resolve_hyp.
+  eexists; intros; instantiate (1:=fun _ x => x); reflexivity.
+  eexists; intros; eapply decode_block_app.
+
+  eapply decode_app_assoc.
+  eapply decode_app_l.
+
+  eapply decode_resolve_hyp.
+  eexists; intros; instantiate (1:=fun _ x => x); reflexivity.
+  eexists; intros; eapply decode_block_app.
+
+  eapply decode_resolve_hyp.
+  eexists; intros; instantiate (1:=fun prev proj =>
+                                     let (prev', f2) := prev in
+                                     let (_, f1)     := prev' in
+                                     Build_SSRecord f1 f2 proj).
+  destruct data; reflexivity.
+  eexists; intros; eapply decode_block_app.
+Defined.
