src/Common/Enumerable.v
@@ -1,0 +1,182 @@
+Require Import Coq.Lists.List.
+Require Import Fiat.Common.List.Operations.
+Require Import Fiat.Common.List.ListFacts.
+Require Import Fiat.Common.StringFacts.
+Require Import Fiat.Common.Equality.
+
+Set Implicit Arguments.
+
+Class Enumerable A
+  := { enumerate : list A;
+       enumerate_correct : forall x, List.In x enumerate }.
+
+Global Arguments enumerate A {_}.
+
+Section enum.
+  Context {A B : Type} (beq : B -> B -> bool).
+
+  Definition enumerate_fun_beq (enumerate : list A) (f g : A -> B)
+  : bool
+    := EqNat.beq_nat (List.length (List.filter (fun x => negb (beq (f x) (g x))) enumerate)) 0.
+
+  Definition enumerate_fun_bl_in
+             (bl : forall x y, beq x y = true -> x = y)
+             (enumerate : list A) (f g : A -> B)
+  : enumerate_fun_beq enumerate f g = true -> forall x, List.In x enumerate -> f x = g x.
+  Proof.
+    unfold enumerate_fun_beq.
+    intros H x H'.
+    apply EqNat.beq_nat_true in H.
+    apply bl.
+    destruct (beq (f x) (g x)) eqn:Heq; [ reflexivity | exfalso ].
+    apply Bool.negb_true_iff in Heq.
+    match type of H with
+      | context[List.filter ?f ?ls]
+        => pose proof (proj2 (@List.filter_In _ f x ls) (conj H' Heq)) as H'';
+          destruct (List.filter f ls)
+    end.
+    { simpl in *.
+      destruct H''. }
+    { simpl in *; omega. }
+  Qed.
+
+  Definition enumerate_fun_bl
+             (bl : forall x y, beq x y = true -> x = y)
+             (enumerate : list A)
+             (enumerate_bl : forall x, List.In x enumerate)
+             (f g : A -> B)
+  : enumerate_fun_beq enumerate f g = true -> forall x, f x = g x.
+  Proof.
+    intros; eapply enumerate_fun_bl_in; try eassumption; trivial.
+  Qed.
+
+  Definition enumerate_fun_false_lb_in
+             (lb : forall x y, x = y -> beq x y = true)
+             (enumerate : list A) (f g : A -> B)
+  : enumerate_fun_beq enumerate f g = false -> { x | List.In x enumerate /\ f x <> g x }.
+  Proof.
+    induction enumerate as [|y ys IHys];
+    unfold enumerate_fun_beq in *; simpl in *;
+    intros H.
+    { exfalso; clear -H; abstract discriminate. }
+    { destruct (beq (f y) (g y)) eqn:Heq; simpl in *.
+      { specialize (IHys H).
+        exists (proj1_sig IHys); split; [ right | ];
+        apply (proj2_sig IHys). }
+      { exists y.
+        split; [ left; reflexivity | ].
+        intro H'.
+        apply lb in H'.
+        clear -H' Heq.
+        generalize dependent (beq (f y) (g y)); clear; intros.
+        abstract congruence. } }
+  Defined.
+
+  Definition enumerate_fun_false_lb
+             (lb : forall x y, x = y -> beq x y = true)
+             (enumerate : list A)
+             (f g : A -> B)
+  : enumerate_fun_beq enumerate f g = false -> { x | f x <> g x }.
+  Proof.
+    intro H.
+    eexists (proj1_sig (enumerate_fun_false_lb_in lb enumerate f g H)).
+    apply (proj2_sig (enumerate_fun_false_lb_in lb enumerate f g H)).
+  Defined.
+
+  Definition enumerate_fun_lb
+             (lb : forall x y, x = y -> beq x y = true)
+             (enumerate : list A)
+             (f g : A -> B)
+  : (forall x, f x = g x) -> enumerate_fun_beq enumerate f g = true.
+  Proof.
+    destruct (enumerate_fun_beq enumerate f g) eqn:Heq; [ reflexivity | ].
+    intro H; exfalso.
+    apply enumerate_fun_false_lb in Heq; [ | assumption.. ].
+    destruct Heq; eauto with nocore.
+  Qed.
+End enum.
+
+Section enumerable.
+  Context {A} {H : Enumerable A} {B} (beq : B -> B -> bool).
+
+  Definition enumerable_fun_beq : (A -> B) -> (A -> B) -> bool
+    := enumerate_fun_beq beq (enumerate A).
+  Definition enumerable_fun_bl
+             (bl : forall x y, beq x y = true -> x = y)
+             (f g : A -> B)
+  : enumerable_fun_beq f g = true -> forall x, f x = g x
+    := enumerate_fun_bl beq bl (enumerate A) enumerate_correct f g.
+  Definition enumerable_fun_false_lb
+             (lb : forall x y, x = y -> beq x y = true)
+             (f g : A -> B)
+  : enumerable_fun_beq f g = false -> { x | f x <> g x }
+    := enumerate_fun_false_lb beq lb (enumerate A) f g.
+  Definition enumerable_fun_lb
+             (lb : forall x y, x = y -> beq x y = true)
+             (f g : A -> B)
+  : (forall x, f x = g x) -> enumerable_fun_beq f g = true
+    := enumerate_fun_lb beq lb (enumerate A) f g.
+End enumerable.
+
+Scheme Equality for unit.
+Definition unit_bl := internal_unit_dec_bl.
+Definition unit_lb := internal_unit_dec_lb.
+
+Local Ltac t bl :=
+  abstract (
+      intro x; apply (list_in_bl bl); revert x;
+      repeat intros []; simpl; try reflexivity
+    ).
+
+Global Instance enumerable_unit : Enumerable unit
+  := { enumerate := tt::nil }.
+Proof. t unit_bl. Defined.
+
+Global Instance enumerable_Empty_set : Enumerable Empty_set
+  := { enumerate := nil }.
+Proof. intros []. Defined.
+
+Global Instance enumerable_True : Enumerable True
+  := { enumerate := I::nil }.
+Proof. intros []; left; reflexivity. Defined.
+
+Global Instance enumerable_False : Enumerable False
+  := { enumerate := nil }.
+Proof. intros []. Defined.
+
+Global Instance enumerable_bool : Enumerable bool
+  := { enumerate := true::false::nil }.
+Proof. t (@bool_bl). Defined.
+
+Global Instance enumerable_sum `{Enumerable A, Enumerable B} : Enumerable (A + B)
+  := { enumerate := List.map inl (enumerate A) ++ List.map inr (enumerate B) }.
+Proof.
+  intros [x|x]; apply in_or_app; [ left | right ];
+  apply in_map;
+  apply enumerate_correct.
+Defined.
+
+Global Instance enumerable_prod `{Enumerable A, Enumerable B} : Enumerable (A * B)
+  := { enumerate := List.flat_map (fun a => List.map (pair a) (enumerate B)) (enumerate A) }.
+Proof.
+  intros [a b].
+  apply List.in_flat_map.
+  exists a; split.
+  { apply enumerate_correct. }
+  { apply in_map;
+    apply enumerate_correct. }
+Defined.
+
+Definition enumerate_ascii : list Ascii.ascii
+  := List.map Ascii.ascii_of_nat (up_to 256).
+
+Global Instance enumerable_ascii : Enumerable Ascii.ascii
+  := { enumerate := enumerate_ascii }.
+Proof.
+  intro x.
+  abstract (
+      rewrite <- (Ascii.ascii_nat_embedding x);
+      unfold enumerate_ascii;
+      apply List.in_map, in_up_to, nat_of_ascii_small
+    ).
+Defined.
