src/Common/Wf.v
@@ -2,6 +2,10 @@
 Require Export Fiat.Common.Coq__8_4__8_5__Compat.
 Require Import Coq.Setoids.Setoid Coq.Program.Program Coq.Program.Wf Coq.Arith.Wf_nat Coq.Classes.Morphisms Coq.Init.Wf.
 Require Import Fiat.Common.Telescope.Core.
+Require Import Fiat.Common.Telescope.Instances.
+Require Import Fiat.Common.Telescope.Equality.
+Require Import Fiat.Common.
+Require Import Fiat.Common.Equality.
 
 Set Implicit Arguments.
 
@@ -211,6 +215,168 @@ Local Arguments flatten_forall_eq_relation / .
 Local Arguments flatten_append_forall / .
 
 Local Notation type_of x := ((fun T (y : T) => T) _ x).
+
+Section FixVTransfer.
+  Context A (B B' : A -> Telescope)
+          (f0 : forall a, flattenT_sig (B a) -> flattenT_sig (B' a))
+          (g0 : forall a, flattenT_sig (B' a) -> flattenT_sig (B a))
+          (sect : forall a x, g0 a (f0 a x) = x)
+          (R : A -> A -> Prop) (Rwf : well_founded R)
+          (P : forall a, flattenT (B a) Type).
+
+  Let P' : forall a, flattenT (B' a) Type
+    := fun a => flattenT_unapply (fun x => flattenT_apply (P a) (g0 _ x)).
+
+  Local Notation FixV := (@Fix A R Rwf (fun a : A => flatten_forall (P a))).
+  Local Notation FixV' := (@Fix A R Rwf (fun a : A => flatten_forall (P' a))).
+
+  Section F.
+    Context (F : forall x : A, (forall y : A, R y x -> flatten_forall (P y)) -> flatten_forall (P x)).
+
+    Let transfer
+    : forall y,
+        flatten_forall
+          (flattenT_unapply
+             (fun x : flattenT_sig (B y) => flattenT_apply (P' y) (f0 y x)))
+        -> flatten_forall (P y).
+    Proof.
+      intro y.
+      refine (flatten_forall_eq_rect
+                (transitivity
+                   ((_ : Proper (pointwise_relation _ _ ==> _) flattenT_unapply)
+                      _ _
+                      (fun x' => transitivity
+                                   (symmetry (flattenT_apply_unapply _ _))
+                                   (f_equal (flattenT_apply _) (sect _ _))))
+                   (symmetry (flattenT_unapply_apply _)))).
+    Defined.
+
+    Let transfer'
+    : forall a,
+        flatten_forall (P a)
+        -> flatten_forall (P' a).
+    Proof.
+      intro a.
+      refine (fun f' => flatten_forall_unapply (fun x' => flatten_forall_apply f' (g0 _ x'))).
+    Defined.
+
+    Let untransfer'
+    : forall a,
+        flatten_forall (P' a)
+        -> flatten_forall (P a).
+    Proof.
+      intro a.
+      refine (fun f' => _).
+      refine (transfer
+                _
+                (flatten_forall_unapply (fun x => flatten_forall_apply f' (f0 _ x)))).
+    Defined.
+
+    Let F' : forall x : A, (forall y : A, R y x -> flatten_forall (P' y)) -> flatten_forall (P' x)
+      := fun a F' => transfer' _ (@F a (fun y pf => transfer _ (flatten_forall_unapply (fun x => flatten_forall_apply (F' y pf) (f0 _ x))))).
+
+
+    Context (F_ext : forall x (f g : forall y, R y x -> flatten_forall (P y)),
+                       (forall y (p : R y x), flatten_forall_eq (f y p) (g y p))
+                       -> flatten_forall_eq (@F x f) (@F x g)).
+
+    Lemma F'_ext
+    : forall x (f g : forall y, R y x -> flatten_forall (P' y)),
+        (forall y (p : R y x), flatten_forall_eq (f y p) (g y p))
+        -> flatten_forall_eq (@F' x f) (@F' x g).
+    Proof.
+      intros x f' g' IH.
+      subst F' transfer transfer'; cbv beta.
+      apply (_ : Proper (forall_relation _ ==> _) flatten_forall_unapply); intro.
+      apply flatten_forall_apply_Proper.
+      apply F_ext; intros.
+      refine ((_ : Proper (flatten_forall_eq ==> _) (@flatten_forall_eq_rect _ _ _ _)) _ _ _).
+      apply (_ : Proper (forall_relation _ ==> _) flatten_forall_unapply); intro.
+      apply flatten_forall_apply_Proper.
+      apply IH.
+    Qed.
+
+    Definition FixV_transfer_eq
+               a
+    : flatten_forall_eq (@FixV F a) (untransfer' _ (@FixV' F' a)).
+    Proof.
+      induction (Rwf a).
+      rewrite FixV_eq by eauto with nocore.
+      etransitivity_rev _.
+      { unfold transfer, untransfer'; cbv beta.
+        apply flatten_forall_eq_rect_Proper, flatten_forall_unapply_Proper; intro.
+        apply flatten_forall_apply_Proper.
+        rewrite FixV_eq by auto using F'_ext with nocore.
+        reflexivity. }
+      etransitivity.
+      { apply F_ext; intros.
+        set_evars.
+        match goal with
+          | [ H : forall y r, flatten_forall_eq _ _ |- _ ] => rewrite H by assumption
+        end.
+        match goal with
+          | [ |- ?R ?a (?e ?x ?y) ]
+            => revert x y
+        end.
+        match goal with
+          | [ H := ?e |- _ ] => is_evar e; subst H
+        end.
+        match goal with
+          | [ |- forall x y, ?R (@?LHS x y) (?RHS x y) ]
+            => unify LHS RHS; cbv beta
+        end.
+        reflexivity. }
+      lazymatch goal with
+        | [ |- appcontext[FixV' ?F] ]
+          => generalize (FixV' F)
+      end.
+      subst F'; cbv beta.
+      subst untransfer' transfer transfer'; cbv beta.
+      intro.
+      rewrite flatten_forall_eq_rect_trans.
+      match goal with
+        | [ |- appcontext[flatten_forall_eq_rect
+                            (flattenT_unapply_Proper ?P ?Q ?H)
+                            (flatten_forall_unapply ?f)] ]
+          => rewrite (@flatten_forall_eq_rect_flattenT_unapply_Proper _ P Q H f)
+      end.
+      etransitivity_rev _.
+      { apply flatten_forall_eq_rect_Proper.
+        apply flatten_forall_unapply_Proper; intro.
+        match goal with
+          | [ |- appcontext[@transitivity _ (@eq ?A) ?P] ]
+            => change (@transitivity _ (@eq ?A) P) with (@eq_trans A)
+        end.
+        match goal with
+          | [ |- appcontext[@symmetry _ (@eq ?A) ?P] ]
+            => change (@symmetry _ (@eq ?A) P) with (@eq_sym A)
+        end.
+        set_evars.
+        rewrite @transport_pp.
+        match goal with
+          | [ |- appcontext G[eq_rect _ (fun T => T) (flatten_forall_apply (flatten_forall_unapply ?k) ?x0) _ (eq_sym (flattenT_apply_unapply ?f1 ?x0))] ]
+            => let H := fresh in
+               pose proof (@eq_rect_symmetry_flattenT_apply_unapply _ f1 x0 k) as H;
+                 cbv beta in H |- *;
+                 let RHS := match type of H with _ = ?RHS => constr:RHS end in
+                 let LHS := match type of H with ?LHS = _ => constr:LHS end in
+                 let G' := context G[LHS] in
+                 change G';
+                   rewrite H;
+                   clear H
+        end.
+        match goal with
+          | [ |- context[f_equal _ ?p] ]
+            => destruct p; unfold f_equal; simpl @eq_rect
+        end.
+        subst_body.
+        reflexivity. }
+      rewrite flatten_forall_eq_rect_symmetry_flattenT_unapply_apply.
+      apply F_ext; intros.
+      reflexivity.
+    Qed.
+  End F.
+End FixVTransfer.
 
 Section Fix_rect.
   Context (A : Type).
